%!TEX program = lualatex
\documentclass{article}
\usepackage{physics, amsmath, amsfonts, empheq, mathtools, booktabs, hyperref, simpler-wick, tikz-feynman, slashed}
\usepackage[style=nature, autocite = inline]{biblatex}
\usepackage[margin=1in]{geometry}

\setlength{\parindent}{0pt}
\numberwithin{equation}{section}

\newcommand*\widefbox[1]{\fbox{\hspace{2em}#1\hspace{2em}}}
\newcommand{\normord}[1]{:\mathrel{#1}:}

\title{Path Integral Quantum Field Theory}
\author{Mathias Driesse}

\begin{document}

\maketitle

\section{Gaussian Integrals}

The General Gaussian integral, for a complex, symmetric $n\times n$ matrix $A$ such that $\Re A \geq 0$ and the eigenvalues $a_i$ of $A$ are nonzero, is given by 

\begin{empheq}[box=\widefbox]{align}
    Z_A(b) = \int d^nx \exp\left(-\frac{1}{2} \sum_{i,j = 1}^n x_i A_{ij}x_j + \sum_{i=1}^n b_i x_i\right) = (2\pi)^{n/2} (\det A)^{-1/2} \exp\left(\frac{1}{2}\sum_{i,j = 1}^n b_i A_{ij}^{-1}b_j \right).
\end{empheq}

Let $\mu$ be a measure in $\mathbb{R}^n$; we define the expectation value

\begin{equation}
\begin{aligned}
    \ev{F}_\mu &= \int d\mu(x)F(x) \\
    &= \int d^nx\, \Omega(x)F(x).
\end{aligned}
\end{equation}

The measure is normalized so that 
\begin{equation}
    \int d\mu(x) = 1.
\end{equation}

We define the generating function 
\begin{equation}
    Z_\mu(b) = \ev{e^{(b,x)}}_\mu = \int d\mu(x) \exp\left(\sum_{i=1}^n b_i x_i\right),
\end{equation}

which is a function of the $n$-dimensional vector $b$ and the measure $\mu$. The integrand can be expanded
\begin{equation}
    \exp\left(\sum_{i=1}^n b_i x_i\right) = \sum_{\ell=0}^\infty \frac{1}{\ell!} \sum_{i_1 \cdots i_\ell = 1}^n b_{i_1} \cdots b_{i_\ell} x_{i_1} \cdots x_{i_\ell}.
\end{equation}
Therefore, substituting the definition of the correlator
\begin{equation}
    \ev{x_{i_1} \cdots x_{i_\ell}}_\mu = \int d\mu(x) x_{i_1} \cdots x_{i_\ell}
\end{equation}
we obtain 
\begin{equation}
    Z_\mu(b) = \sum_{\ell=0}^\infty \frac{1}{\ell!} \sum_{i_1 \cdots i_\ell = 1}^n b_{i_1} \cdots b_{i_\ell} \ev{x_{i_1} \cdots x_{i_\ell}}_\mu.
\end{equation}
Furthermore, it is useful to notice that
\begin{equation}
    \pdv{b_k} Z_\mu(b) = \int d\mu(x)x_k \exp\left(\sum_{i=1}^n b_i x_i\right),
\end{equation}
which allows the correlaters to be written as
\begin{equation}
    \ev{x_{i_1} \cdots x_{i_\ell}}_\mu = \pdv{b_{i_1}} \cdots \pdv{b_{i_\ell}} Z_\mu(b) \eval_{b=0}.
\end{equation}

Let us consder the Gaussian measure
\begin{equation} \label{eq:gaussian_measure}
    d\mu_0(x) = d^nx\, \Omega_0(x) = d^nx \, \mathcal{N}_0 \exp\left(-\frac{1}{2}\sum_{i,j=0}^n x_i A_{ij}x_j\right),
\end{equation}
where the normalization $\mathcal{N}_0$ is fixed by the normalization of the measure:
\begin{equation}
    \mathcal{N}_0 = (2\pi)^{-n/2} (\det A)^{1/2}.
\end{equation}
The generating function in this case can be readily computed using the boxed equation above:
\begin{equation}
    Z(b) = \frac{Z_A(b)}{Z_A(0)} = \exp\left(\frac{1}{2}\sum_{i,j = 1}^n b_i A_{ij}^{-1} b_j\right).
\end{equation}
In the future, we will drop any subscript $A$ when referring to a Gaussian measure for simplicity. And therefore, defining $\Delta_{ij} = A_{ij}^{-1}$, 
\begin{empheq}[box=\widefbox]{align} \label{eq:correlator}
    \ev{x_{i_1}\cdots x_{i_\ell} }_0 = \pdv{b_{i_1}} \cdots \pdv{b_{i_\ell}} \eval{\exp\left(\frac{1}{2}\sum_{i,j=1}^n b_i \Delta_{ij} b_j\right)}_{b=0}.
\end{empheq}

\subsection{Wick's Theorem}

Let us start with a couple explicit examples, which we will compute in full detail in order to get familiar with the algebraic manipulations.

\textbf{One-point function}: Let $k$ be an integer between 1 and $n$, we have 
\begin{equation}
\begin{aligned}
    \ev{x_k}_0 &= \pdv{b_k} \eval{\exp\left(\frac{1}{2}\sum_{i,j = 1}^n b_i \Delta_{ij} b_j \right)}_{b=0} \\
    &= \left(\frac{1}{2}\sum_{j=1}^n \Delta_{kj}b_j + \frac{1}{2}\sum_{i=1}^n b_i \Delta_{ik} \right)\eval{\exp\left(\frac{1}{2}\sum_{i,j = 1}^n b_i \Delta_{ij} b_j \right)}_{b=0} \\
    &= \left(\sum_{j=1}^n \Delta_{kj}b_j\right)\eval{\exp\left(\frac{1}{2}\sum_{i,j = 1}^n b_i \Delta_{ij} b_j \right)}_{b=0} \\
    &= 0,
\end{aligned}
\end{equation}
where the last equality comes from the fact that the expression is linear in $b$, and we need to set $b=0$.

\textbf{Two-point function}: We now consider a pair of indices $k$, $l$, and compute
\begin{equation}
\begin{aligned}
    \ev{x_k x_l}_0 &= \pdv{b_l} \pdv{b_k} \eval{\exp\left(\frac{1}{2}\sum_{i,j = 1}^n b_i \Delta_{ij} b_j \right)}_{b=0} \\
    &= \left[\Delta_{kl} + \left(\sum_{j=1}^n \Delta_{kj} b_j \right) \left(\sum_{m=1}^n \Delta_{lm} b_m \right)\right] \eval{\exp\left(\frac{1}{2}\sum_{i,j = 1}^n b_i \Delta_{ij} b_j \right)}_{b=0} \\
    &= \Delta_{kl}
\end{aligned}
\end{equation}

Thus, the generating function $Z(b)$ provides a systematic way to compute all correlators for a multi-dimensional Gaussian distribution. Having understood the general rule for such a process, we can generate a recipe to compute $\ev{x_{i_1} \cdots x_{i_\ell}}_0$, known as \textit{Wick's Theorem}:
\begin{itemize}
    \item Write down each $x_{i_1} \cdots x_{i_\ell}$ and organize them pairwise $(i_p, i_q)$. Note that if $\ell$ must be even for the correlator to be non-zero.
    \item There are $(\ell - 1)\times(\ell-3) \times \cdots \times 3 \times 1$ ways of doing this. Sum over all of these possible pairings.
    \item To each pair $(i_p, i_q)$ associate a factor $\Delta_{i_p i_q}$.
\end{itemize}

Let us revisit our result for the \textbf{two-point function}: for $\ev{x_{i_1} x_{i_2}}_0$, there is only one possible pairing $(i_1, i_2)$. Therefore
\begin{equation}
    \ev{x_{i_1} x_{i_2}}_0 = \Delta_{i_1 i_2}.
\end{equation}

\textbf{Four-point function}: For $\ev{x_{i_1} x_{i_2} x_{i_3} x_{i_4}}_0$, there are three different pairings
\begin{equation}
    P=\left\{\left\{\left(i_1, i_2\right),\left(i_3, i_4\right)\right\},\left\{\left(i_1, i_3\right),\left(i_2, i_4\right)\right\},\left\{\left(i_1, i_4\right),\left(i_2, i_3\right)\right\}\right\}
\end{equation}

Wick's theorem then yields 
\begin{equation}
    \ev{x_{i_1} x_{i_2} x_{i_3} x_{i_4}}_0=\Delta_{i_1 i_2} \Delta_{i_3 i_4}+\Delta_{i_1 i_3} \Delta_{i_2 i_4}+\Delta_{i_1 i_4} \Delta_{i_2 i_3}.
\end{equation}

We can also represent these pairings, \textit{Wick contractions}, as should be familiar from canonical quantum field theory:
\begin{equation}
    \ev{x_i x_j}_0 = \Delta_{ij} = \wick{\c x_i \c x_j}
\end{equation}

\subsection{Perturbed Gaussian Measure}

Let us now consider a more complicated measure,
\begin{equation}
    \Omega(x) = \frac{1}{Z(\lambda)}e^{-S(x, \lambda)},
\end{equation}
where the normalization is given as usual by 
\begin{equation}
    Z(\lambda) = \int d^nx e^{-S(x,\lambda)}
\end{equation}
and
\begin{equation}
\begin{aligned}
    S(x, \lambda) &= \frac{1}{2} \sum_{i, j = 1}^n x_i A_{ij}x_j + \lambda V(x) \\
    &= S_0(x) + \lambda V(x).
\end{aligned}
\end{equation}
We call $V(\lambda)$ the potential term, foreshadowing the physics we will be doing using the perturbed Gaussian measure. Furthermore
\begin{equation}
\begin{aligned}
    Z(\lambda) &= \sum_{k=0}^\infty \frac{(-\lambda)^k}{k!} \int d^nx \, V^k(x) \exp\left(-\frac{1}{2} \sum_{i,j=1}^n x_i A_{ij} x_j\right) \\
    &= Z(0) \sum_{k=0}^\infty \frac{(-\lambda)^k}{k!} \ev{V^k(x)}_0,
\end{aligned}
\end{equation}
where in the first line we have expanded the exponential term containing $e^V(x)$ and in the second line used
\begin{equation}
    \ev{F(x)}_0 = \frac{1}{Z(0)} \int d^nx \exp\left(-\frac{1}{2} \sum_{i,j=1}^n x_i A_{ij} x_j\right) F(x),
\end{equation}
and $1/Z(0)$ referring to the normalization constant $\mathcal{N}_0$ from Eq. \ref{eq:gaussian_measure}. Recalling Eq. \ref{eq:correlator}, given that $F(x)$ admits a Taylor expansion
\begin{equation}
    F(x) = \sum_{\ell = 0}^\infty \sum_{i_1 \cdots i_\ell = 1}^n F_{i_1 \cdots i_\ell} x_{i_1} \cdots x_{i_\ell},
\end{equation}
we can define the expectation value of $F$ for a generic measure $\mu$ as 
\begin{equation}
    \ev{F(x)}_\mu = \sum_{\ell = 0}^\infty \sum_{i_1 \cdots i_\ell = 1}^n F_{i_1 \cdots i_\ell} \ev{x_{i_1} \cdots x_{i_\ell}}_\mu;
\end{equation}
for the case of a Gaussian measure we obtain
\begin{equation}
\begin{aligned}
    \ev{F(x)}_0 &= \sum_{\ell = 0}^\infty \sum_{i_1 \cdots i_\ell = 1}^n F_{i_1 \cdots i_\ell} \pdv{b_{i_1}} \cdots \pdv{b_{i_\ell}} \eval{\exp\left(\frac{1}{2}\sum_{i,j=1}^n b_i \Delta_{ij} b_j\right)}_{b=0} \\
    &= F \left(\pdv{b}\right) \eval{\exp\left(\frac{1}{2}\sum_{i,j=1}^n b_i \Delta_{ij} b_j\right)}_{b=0}.
\end{aligned}
\end{equation}

Thus, returning to our potential term,
\begin{equation}
\begin{aligned}
    \frac{Z(\lambda)}{Z(0)} &= \ev{e^{-\lambda V(x)}}_0 \\
    &= \exp\left[-\lambda V\left(\pdv{b}\right)\right] \eval{\exp\left(\frac{1}{2}\sum_{i,j=1}^n b_i \Delta_{ij} b_j\right)}_{b=0}
\end{aligned}
\end{equation}


\end{document}